code/ecdsap256/Hacl.Spec.P256.Montgomery.fsti
@@ -1,0 +1,44 @@
+module Hacl.Spec.P256.Montgomery
+
+open FStar.Mul
+
+module S = Spec.P256
+
+#set-options "--z3rlimit 50 --fuel 0 --ifuel 0"
+
+///  Montgomery arithmetic for a base field
+
+let fmont_R = pow2 256
+let fmont_R_inv = S.modp_inv2_prime (pow2 256) S.prime
+
+let from_mont (a:int) : S.felem = a * fmont_R_inv % S.prime
+let to_mont   (a:int) : S.felem = a * fmont_R % S.prime
+
+// used in Hacl.Impl.P256.Field
+val lemma_mod_mul_pow256_prime: a:int -> b:int -> Lemma
+  (requires a * pow2 256 % S.prime = b * pow2 256 % S.prime)
+  (ensures  a % S.prime == b % S.prime)
+
+// used in Hacl.Impl.P256.Point
+val lemma_multiplication_not_mod_prime: a:S.felem ->
+  Lemma (a * fmont_R_inv % S.prime == 0 <==> a == 0)
+
+val lemma_to_from_mont_id: a:S.felem -> Lemma (from_mont (to_mont a) == a)
+val lemma_from_to_mont_id: a:S.felem -> Lemma (to_mont (from_mont a) == a)
+
+val fmont_mul_lemma: a:S.felem -> b:S.felem ->
+  Lemma (S.fmul (from_mont a) (from_mont b) = from_mont ((a * b * fmont_R_inv) % S.prime))
+
+val fmont_add_lemma: a:S.felem -> b:S.felem ->
+  Lemma (S.fadd (from_mont a) (from_mont b) = from_mont ((a + b) % S.prime))
+
+val fmont_sub_lemma: a:S.felem -> b:S.felem ->
+  Lemma (S.fsub (from_mont a) (from_mont b) = from_mont ((a - b) % S.prime))
+
+
+///  Montgomery arithmetic for a scalar field
+
+// used in Hacl.Impl.P256.Scalar
+val lemma_mod_mul_pow256_order: a:int -> b:int -> Lemma
+  (requires a * pow2 256 % S.order = b * pow2 256 % S.order)
+  (ensures  a % S.order == b % S.order)
